examples/Examples/ProgramsProofs/InsertionSort.lean
@@ -10,6 +10,7 @@ end expect
 
 
 expect error {{{ insertSortedNoProof }}}
+  -- TODO arr.swap now uses auto params instead of Fin, check text
   def insertSorted [Ord α] (arr : Array α) (i : Fin arr.size) : Array α :=
     match i with
     | ⟨0, _⟩ => arr
@@ -19,23 +20,23 @@ expect error {{{ insertSortedNoProof }}}
       match Ord.compare arr[i'] arr[i] with
       | .lt | .eq => arr
       | .gt =>
-        insertSorted (arr.swap ⟨i', by assumption⟩ i) ⟨i', by simp [*]⟩
+        insertSorted (arr.swap i' i) ⟨i', by simp [*]⟩
 message
 "unsolved goals
 α : Type ?u.7
 inst✝ : Ord α
 arr : Array α
-i : Fin (Array.size arr)
+i : Fin arr.size
 i' : Nat
-isLt✝ : i' + 1 < Array.size arr
-⊢ i' < Array.size arr"
+isLt✝ : i' + 1 < arr.size
+⊢ i' < arr.size"
 end expect
 
 
 expect info {{{ lt_of_succ_lt_type }}}
   #check Nat.lt_of_succ_lt
 message
-"Nat.lt_of_succ_lt {n m : Nat} (a✝ : Nat.succ n < m) : n < m"
+"Nat.lt_of_succ_lt {n m : Nat} : n.succ < m → n < m"
 end expect
 
 -- Precondition: array positions 0 .. i-1 are sorted
@@ -50,7 +51,7 @@ book declaration {{{ insertSorted }}}
       match Ord.compare arr[i'] arr[i] with
       | .lt | .eq => arr
       | .gt =>
-        insertSorted (arr.swap ⟨i', by assumption⟩ i) ⟨i', by simp [*]⟩
+        insertSorted (arr.swap i' i) ⟨i', by simp [*]⟩
 stop book declaration
 
 -- theorem insert_sorted_size_eq' [Ord α] (len : Nat) (i : Nat) :
@@ -82,29 +83,20 @@ case succ
 α : Type u_1
 inst✝ : Ord α
 arr : Array α
-i : Fin (Array.size arr)
+i : Fin arr.size
 j' : Nat
-ih : ∀ (isLt : j' < Array.size arr), Array.size (insertSorted arr { val := j', isLt := isLt }) = Array.size arr
-isLt : Nat.succ j' < Array.size arr
-⊢ Array.size
-      (match compare arr[j'] arr[{ val := Nat.succ j', isLt := isLt }] with
+ih : ∀ (isLt : j' < arr.size), (insertSorted arr ⟨j', isLt⟩).size = arr.size
+isLt : j' + 1 < arr.size
+⊢ (match compare arr[j'] arr[j' + 1] with
       | Ordering.lt => arr
       | Ordering.eq => arr
-      | Ordering.gt =>
-        insertSorted
-          (Array.swap arr { val := j', isLt := (_ : j' < Array.size arr) } { val := Nat.succ j', isLt := isLt })
-          { val := j',
-            isLt :=
-              (_ :
-                j' <
-                  Array.size
-                    (Array.swap arr { val := j', isLt := (_ : j' < Array.size arr) }
-                      { val := Nat.succ j', isLt := isLt })) }) =
-    Array.size arr"
+      | Ordering.gt => insertSorted (arr.swap j' (j' + 1) ⋯ ⋯) ⟨j', ⋯⟩).size =
+    arr.size"
 end expect
 
 
 expect error {{{ insert_sorted_size_eq_1 }}}
+  -- TODO describe elided proofs in text - these appeared here
   theorem insert_sorted_size_eq [Ord α] (arr : Array α) (i : Fin arr.size) :
       (insertSorted arr i).size = arr.size := by
     match i with
@@ -120,51 +112,42 @@ case succ.h_1
 α : Type u_1
 inst✝ : Ord α
 arr : Array α
-i : Fin (Array.size arr)
+i : Fin arr.size
 j' : Nat
-ih : ∀ (isLt : j' < Array.size arr), Array.size (insertSorted arr { val := j', isLt := isLt }) = Array.size arr
-isLt : Nat.succ j' < Array.size arr
+ih : ∀ (isLt : j' < arr.size), (insertSorted arr ⟨j', isLt⟩).size = arr.size
+isLt : j' + 1 < arr.size
 x✝ : Ordering
-heq✝ : compare arr[j'] arr[{ val := Nat.succ j', isLt := isLt }] = Ordering.lt
-⊢ Array.size arr = Array.size arr
+heq✝ : compare arr[j'] arr[j' + 1] = Ordering.lt
+⊢ arr.size = arr.size
 
 case succ.h_2
 α : Type u_1
 inst✝ : Ord α
 arr : Array α
-i : Fin (Array.size arr)
+i : Fin arr.size
 j' : Nat
-ih : ∀ (isLt : j' < Array.size arr), Array.size (insertSorted arr { val := j', isLt := isLt }) = Array.size arr
-isLt : Nat.succ j' < Array.size arr
+ih : ∀ (isLt : j' < arr.size), (insertSorted arr ⟨j', isLt⟩).size = arr.size
+isLt : j' + 1 < arr.size
 x✝ : Ordering
-heq✝ : compare arr[j'] arr[{ val := Nat.succ j', isLt := isLt }] = Ordering.eq
-⊢ Array.size arr = Array.size arr
+heq✝ : compare arr[j'] arr[j' + 1] = Ordering.eq
+⊢ arr.size = arr.size
 
 case succ.h_3
 α : Type u_1
 inst✝ : Ord α
 arr : Array α
-i : Fin (Array.size arr)
+i : Fin arr.size
 j' : Nat
-ih : ∀ (isLt : j' < Array.size arr), Array.size (insertSorted arr { val := j', isLt := isLt }) = Array.size arr
-isLt : Nat.succ j' < Array.size arr
+ih : ∀ (isLt : j' < arr.size), (insertSorted arr ⟨j', isLt⟩).size = arr.size
+isLt : j' + 1 < arr.size
 x✝ : Ordering
-heq✝ : compare arr[j'] arr[{ val := Nat.succ j', isLt := isLt }] = Ordering.gt
-⊢ Array.size
-      (insertSorted
-        (Array.swap arr { val := j', isLt := (_ : j' < Array.size arr) } { val := Nat.succ j', isLt := isLt })
-        { val := j',
-          isLt :=
-            (_ :
-              j' <
-                Array.size
-                  (Array.swap arr { val := j', isLt := (_ : j' < Array.size arr) }
-                    { val := Nat.succ j', isLt := isLt })) }) =
-    Array.size arr"
+heq✝ : compare arr[j'] arr[j' + 1] = Ordering.gt
+⊢ (insertSorted (arr.swap j' (j' + 1) ⋯ ⋯) ⟨j', ⋯⟩).size = arr.size"
 end expect
 
 
 expect error {{{ insert_sorted_size_eq_2 }}}
+  -- TODO big in-bounds proofs are now elided - check text
   theorem insert_sorted_size_eq [Ord α] (arr : Array α) (i : Fin arr.size) :
       (insertSorted arr i).size = arr.size := by
     match i with
@@ -180,23 +163,13 @@ case succ.h_3
 α : Type u_1
 inst✝ : Ord α
 arr : Array α
-i : Fin (Array.size arr)
+i : Fin arr.size
 j' : Nat
-ih : ∀ (isLt : j' < Array.size arr), Array.size (insertSorted arr { val := j', isLt := isLt }) = Array.size arr
-isLt : Nat.succ j' < Array.size arr
+ih : ∀ (isLt : j' < arr.size), (insertSorted arr ⟨j', isLt⟩).size = arr.size
+isLt : j' + 1 < arr.size
 x✝ : Ordering
-heq✝ : compare arr[j'] arr[{ val := Nat.succ j', isLt := isLt }] = Ordering.gt
-⊢ Array.size
-      (insertSorted
-        (Array.swap arr { val := j', isLt := (_ : j' < Array.size arr) } { val := Nat.succ j', isLt := isLt })
-        { val := j',
-          isLt :=
-            (_ :
-              j' <
-                Array.size
-                  (Array.swap arr { val := j', isLt := (_ : j' < Array.size arr) }
-                    { val := Nat.succ j', isLt := isLt })) }) =
-    Array.size arr"
+heq✝ : compare arr[j'] arr[j' + 1] = Ordering.gt
+⊢ (insertSorted (arr.swap j' (j' + 1) ⋯ ⋯) ⟨j', ⋯⟩).size = arr.size"
 end expect
 
 
@@ -216,26 +189,13 @@ case succ.h_3
 α : Type u_1
 inst✝ : Ord α
 j' : Nat
-ih :
-  ∀ (arr : Array α),
-    Fin (Array.size arr) →
-      ∀ (isLt : j' < Array.size arr), Array.size (insertSorted arr { val := j', isLt := isLt }) = Array.size arr
+ih : ∀ (arr : Array α), Fin arr.size → ∀ (isLt : j' < arr.size), (insertSorted arr ⟨j', isLt⟩).size = arr.size
 arr : Array α
-i : Fin (Array.size arr)
-isLt : Nat.succ j' < Array.size arr
+i : Fin arr.size
+isLt : j' + 1 < arr.size
 x✝ : Ordering
-heq✝ : compare arr[j'] arr[{ val := Nat.succ j', isLt := isLt }] = Ordering.gt
-⊢ Array.size
-      (insertSorted
-        (Array.swap arr { val := j', isLt := (_ : j' < Array.size arr) } { val := Nat.succ j', isLt := isLt })
-        { val := j',
-          isLt :=
-            (_ :
-              j' <
-                Array.size
-                  (Array.swap arr { val := j', isLt := (_ : j' < Array.size arr) }
-                    { val := Nat.succ j', isLt := isLt })) }) =
-    Array.size arr"
+heq✝ : compare arr[j'] arr[j' + 1] = Ordering.gt
+⊢ (insertSorted (arr.swap j' (j' + 1) ⋯ ⋯) ⟨j', ⋯⟩).size = arr.size"
 end expect
 
 
@@ -249,8 +209,7 @@ message
 α : Type u_1
 inst✝ : Ord α
 len i : Nat
-⊢ ∀ (arr : Array α) (isLt : i < Array.size arr),
-    Array.size arr = len → Array.size (insertSorted arr { val := i, isLt := isLt }) = len"
+⊢ ∀ (arr : Array α) (isLt : i < arr.size), arr.size = len → (insertSorted arr ⟨i, isLt⟩).size = len"
 end expect
 
 
@@ -267,8 +226,7 @@ case zero
 α : Type u_1
 inst✝ : Ord α
 len : Nat
-⊢ ∀ (arr : Array α) (isLt : Nat.zero < Array.size arr),
-    Array.size arr = len → Array.size (insertSorted arr { val := Nat.zero, isLt := isLt }) = len"
+⊢ ∀ (arr : Array α) (isLt : 0 < arr.size), arr.size = len → (insertSorted arr ⟨0, isLt⟩).size = len"
 end expect
 
 expect error {{{ insert_sorted_size_eq_redo_1b }}}
@@ -284,11 +242,8 @@ case succ
 α : Type u_1
 inst✝ : Ord α
 len i' : Nat
-ih :
-  ∀ (arr : Array α) (isLt : i' < Array.size arr),
-    Array.size arr = len → Array.size (insertSorted arr { val := i', isLt := isLt }) = len
-⊢ ∀ (arr : Array α) (isLt : Nat.succ i' < Array.size arr),
-    Array.size arr = len → Array.size (insertSorted arr { val := Nat.succ i', isLt := isLt }) = len"
+ih : ∀ (arr : Array α) (isLt : i' < arr.size), arr.size = len → (insertSorted arr ⟨i', isLt⟩).size = len
+⊢ ∀ (arr : Array α) (isLt : i' + 1 < arr.size), arr.size = len → (insertSorted arr ⟨i' + 1, isLt⟩).size = len"
 end expect
 
 
@@ -308,9 +263,9 @@ case zero
 inst✝ : Ord α
 len : Nat
 arr : Array α
-isLt : Nat.zero < Array.size arr
-hLen : Array.size arr = len
-⊢ Array.size arr = len"
+isLt : 0 < arr.size
+hLen : arr.size = len
+⊢ arr.size = len"
 end expect
 
 
@@ -329,11 +284,8 @@ case succ
 α : Type u_1
 inst✝ : Ord α
 len i' : Nat
-ih :
-  ∀ (arr : Array α) (isLt : i' < Array.size arr),
-    Array.size arr = len → Array.size (insertSorted arr { val := i', isLt := isLt }) = len
-⊢ ∀ (arr : Array α) (isLt : Nat.succ i' < Array.size arr),
-    Array.size arr = len → Array.size (insertSorted arr { val := Nat.succ i', isLt := isLt }) = len"
+ih : ∀ (arr : Array α) (isLt : i' < arr.size), arr.size = len → (insertSorted arr ⟨i', isLt⟩).size = len
+⊢ ∀ (arr : Array α) (isLt : i' + 1 < arr.size), arr.size = len → (insertSorted arr ⟨i' + 1, isLt⟩).size = len"
 end expect
 
 
@@ -354,26 +306,14 @@ case succ
 α : Type u_1
 inst✝ : Ord α
 len i' : Nat
-ih :
-  ∀ (arr : Array α) (isLt : i' < Array.size arr),
-    Array.size arr = len → Array.size (insertSorted arr { val := i', isLt := isLt }) = len
+ih : ∀ (arr : Array α) (isLt : i' < arr.size), arr.size = len → (insertSorted arr ⟨i', isLt⟩).size = len
 arr : Array α
-isLt : Nat.succ i' < Array.size arr
-hLen : Array.size arr = len
-⊢ Array.size
-      (match compare arr[i'] arr[{ val := Nat.succ i', isLt := isLt }] with
+isLt : i' + 1 < arr.size
+hLen : arr.size = len
+⊢ (match compare arr[i'] arr[i' + 1] with
       | Ordering.lt => arr
       | Ordering.eq => arr
-      | Ordering.gt =>
-        insertSorted
-          (Array.swap arr { val := i', isLt := (_ : i' < Array.size arr) } { val := Nat.succ i', isLt := isLt })
-          { val := i',
-            isLt :=
-              (_ :
-                i' <
-                  Array.size
-                    (Array.swap arr { val := i', isLt := (_ : i' < Array.size arr) }
-                      { val := Nat.succ i', isLt := isLt })) }) =
+      | Ordering.gt => insertSorted (arr.swap i' (i' + 1) ⋯ ⋯) ⟨i', ⋯⟩).size =
     len"
 end expect
 
@@ -396,53 +336,37 @@ case succ.h_1
 α : Type u_1
 inst✝ : Ord α
 len i' : Nat
-ih :
-  ∀ (arr : Array α) (isLt : i' < Array.size arr),
-    Array.size arr = len → Array.size (insertSorted arr { val := i', isLt := isLt }) = len
+ih : ∀ (arr : Array α) (isLt : i' < arr.size), arr.size = len → (insertSorted arr ⟨i', isLt⟩).size = len
 arr : Array α
-isLt : Nat.succ i' < Array.size arr
-hLen : Array.size arr = len
+isLt : i' + 1 < arr.size
+hLen : arr.size = len
 x✝ : Ordering
-heq✝ : compare arr[i'] arr[{ val := Nat.succ i', isLt := isLt }] = Ordering.lt
-⊢ Array.size arr = len
+heq✝ : compare arr[i'] arr[i' + 1] = Ordering.lt
+⊢ arr.size = len
 
 case succ.h_2
 α : Type u_1
 inst✝ : Ord α
 len i' : Nat
-ih :
-  ∀ (arr : Array α) (isLt : i' < Array.size arr),
-    Array.size arr = len → Array.size (insertSorted arr { val := i', isLt := isLt }) = len
+ih : ∀ (arr : Array α) (isLt : i' < arr.size), arr.size = len → (insertSorted arr ⟨i', isLt⟩).size = len
 arr : Array α
-isLt : Nat.succ i' < Array.size arr
-hLen : Array.size arr = len
+isLt : i' + 1 < arr.size
+hLen : arr.size = len
 x✝ : Ordering
-heq✝ : compare arr[i'] arr[{ val := Nat.succ i', isLt := isLt }] = Ordering.eq
-⊢ Array.size arr = len
+heq✝ : compare arr[i'] arr[i' + 1] = Ordering.eq
+⊢ arr.size = len
 
 case succ.h_3
 α : Type u_1
 inst✝ : Ord α
 len i' : Nat
-ih :
-  ∀ (arr : Array α) (isLt : i' < Array.size arr),
-    Array.size arr = len → Array.size (insertSorted arr { val := i', isLt := isLt }) = len
+ih : ∀ (arr : Array α) (isLt : i' < arr.size), arr.size = len → (insertSorted arr ⟨i', isLt⟩).size = len
 arr : Array α
-isLt : Nat.succ i' < Array.size arr
-hLen : Array.size arr = len
+isLt : i' + 1 < arr.size
+hLen : arr.size = len
 x✝ : Ordering
-heq✝ : compare arr[i'] arr[{ val := Nat.succ i', isLt := isLt }] = Ordering.gt
-⊢ Array.size
-      (insertSorted
-        (Array.swap arr { val := i', isLt := (_ : i' < Array.size arr) } { val := Nat.succ i', isLt := isLt })
-        { val := i',
-          isLt :=
-            (_ :
-              i' <
-                Array.size
-                  (Array.swap arr { val := i', isLt := (_ : i' < Array.size arr) }
-                    { val := Nat.succ i', isLt := isLt })) }) =
-    len"
+heq✝ : compare arr[i'] arr[i' + 1] = Ordering.gt
+⊢ (insertSorted (arr.swap i' (i' + 1) ⋯ ⋯) ⟨i', ⋯⟩).size = len"
 end expect
 
 
@@ -464,25 +388,13 @@ case succ.h_3
 α : Type u_1
 inst✝ : Ord α
 len i' : Nat
-ih :
-  ∀ (arr : Array α) (isLt : i' < Array.size arr),
-    Array.size arr = len → Array.size (insertSorted arr { val := i', isLt := isLt }) = len
+ih : ∀ (arr : Array α) (isLt : i' < arr.size), arr.size = len → (insertSorted arr ⟨i', isLt⟩).size = len
 arr : Array α
-isLt : Nat.succ i' < Array.size arr
-hLen : Array.size arr = len
+isLt : i' + 1 < arr.size
+hLen : arr.size = len
 x✝ : Ordering
-heq✝ : compare arr[i'] arr[{ val := Nat.succ i', isLt := isLt }] = Ordering.gt
-⊢ Array.size
-      (insertSorted
-        (Array.swap arr { val := i', isLt := (_ : i' < Array.size arr) } { val := Nat.succ i', isLt := isLt })
-        { val := i',
-          isLt :=
-            (_ :
-              i' <
-                Array.size
-                  (Array.swap arr { val := i', isLt := (_ : i' < Array.size arr) }
-                    { val := Nat.succ i', isLt := isLt })) }) =
-    len"
+heq✝ : compare arr[i'] arr[i' + 1] = Ordering.gt
+⊢ (insertSorted (arr.swap i' (i' + 1) ⋯ ⋯) ⟨i', ⋯⟩).size = len"
 end expect
 
 namespace Wak
@@ -506,37 +418,23 @@ case succ.h_2
 α : Type u_1
 inst✝ : Ord α
 i' : Nat
-ih :
-  ∀ (arr : Array α) (isLt : i' < Array.size arr),
-    Array.size arr = Array.size (insertSorted arr { val := i', isLt := isLt })
+ih : ∀ (arr : Array α) (isLt : i' < arr.size), arr.size = (insertSorted arr ⟨i', isLt⟩).size
 arr : Array α
-isLt : Nat.succ i' < Array.size arr
+isLt : i' + 1 < arr.size
 x✝ : Ordering
-heq✝ : compare arr[i'] arr[{ val := Nat.succ i', isLt := isLt }] = Ordering.eq
-⊢ Array.size arr = Array.size arr
+heq✝ : compare arr[i'] arr[i' + 1] = Ordering.eq
+⊢ arr.size = arr.size
 
 case succ.h_3
 α : Type u_1
 inst✝ : Ord α
 i' : Nat
-ih :
-  ∀ (arr : Array α) (isLt : i' < Array.size arr),
-    Array.size arr = Array.size (insertSorted arr { val := i', isLt := isLt })
+ih : ∀ (arr : Array α) (isLt : i' < arr.size), arr.size = (insertSorted arr ⟨i', isLt⟩).size
 arr : Array α
-isLt : Nat.succ i' < Array.size arr
+isLt : i' + 1 < arr.size
 x✝ : Ordering
-heq✝ : compare arr[i'] arr[{ val := Nat.succ i', isLt := isLt }] = Ordering.gt
-⊢ Array.size arr =
-    Array.size
-      (insertSorted
-        (Array.swap arr { val := i', isLt := (_ : i' < Array.size arr) } { val := Nat.succ i', isLt := isLt })
-        { val := i',
-          isLt :=
-            (_ :
-              i' <
-                Array.size
-                  (Array.swap arr { val := i', isLt := (_ : i' < Array.size arr) }
-                    { val := Nat.succ i', isLt := isLt })) })"
+heq✝ : compare arr[i'] arr[i' + 1] = Ordering.gt
+⊢ arr.size = (insertSorted (arr.swap i' (i' + 1) ⋯ ⋯) ⟨i', ⋯⟩).size"
 end expect
 end Wak
 
@@ -584,13 +482,27 @@ message
 "fail to show termination for
   insertionSortLoop
 with errors
-argument #4 was not used for structural recursion
+failed to infer structural recursion:
+Not considering parameter α of insertionSortLoop:
+  it is unchanged in the recursive calls
+Not considering parameter #2 of insertionSortLoop:
+  it is unchanged in the recursive calls
+Cannot use parameter arr:
+  the type Array α does not have a `.brecOn` recursor
+Cannot use parameter i:
   failed to eliminate recursive application
-    insertionSortLoop (insertSorted arr { val := i, isLt := h }) (i + 1)
+    insertionSortLoop (insertSorted arr ⟨i, h⟩) (i + 1)
 
-structural recursion cannot be used
 
-failed to prove termination, use `termination_by` to specify a well-founded relation"
+Could not find a decreasing measure.
+The basic measures relate at each recursive call as follows:
+(<, ≤, =: relation proved, ? all proofs failed, _: no proof attempted)
+            arr i #1
+1) 478:6-57   ? ?  ?
+
+#1: arr.size - i
+
+Please use `termination_by` to specify a decreasing measure."
 end expect
 
 namespace Partial
@@ -619,12 +531,13 @@ end Partial
 
 
 expect error {{{ insertionSortLoopProof1 }}}
+  -- TODO syntax change for termination_by - no longer binds args. Check text!
   def insertionSortLoop [Ord α] (arr : Array α) (i : Nat) : Array α :=
     if h : i < arr.size then
       insertionSortLoop (insertSorted arr ⟨i, h⟩) (i + 1)
     else
       arr
-  termination_by insertionSortLoop arr i => arr.size - i
+  termination_by arr.size - i
 message
 "failed to prove termination, possible solutions:
   - Use `have`-expressions to prove the remaining goals
@@ -634,8 +547,8 @@ message
 inst✝ : Ord α
 arr : Array α
 i : Nat
-h : i < Array.size arr
-⊢ Array.size (insertSorted arr { val := i, isLt := h }) - (i + 1) < Array.size arr - i"
+h : i < arr.size
+⊢ (insertSorted arr ⟨i, h⟩).size - (i + 1) < arr.size - i"
 end expect
 
 
@@ -649,7 +562,7 @@ expect warning {{{ insertionSortLoopSorry }}}
       insertionSortLoop (insertSorted arr ⟨i, h⟩) (i + 1)
     else
       arr
-  termination_by insertionSortLoop arr i => arr.size - i
+  termination_by arr.size - i
 message
 "declaration uses 'sorry'"
 end expect
@@ -663,15 +576,15 @@ expect error {{{ insertionSortLoopRw }}}
       insertionSortLoop (insertSorted arr ⟨i, h⟩) (i + 1)
     else
       arr
-termination_by insertionSortLoop arr i => arr.size - i
+termination_by arr.size - i
 message
 "unsolved goals
-α : Type ?u.22173
+α : Type ?u.23737
 inst✝ : Ord α
 arr : Array α
 i : Nat
-h : i < Array.size arr
-⊢ Array.size arr - (i + 1) < Array.size arr - i"
+h : i < arr.size
+⊢ arr.size - (i + 1) < arr.size - i"
 end expect
 
 bookExample type {{{ sub_succ_lt_self_type }}}
@@ -691,7 +604,7 @@ book declaration {{{ insertionSortLoop }}}
       insertionSortLoop (insertSorted arr ⟨i, h⟩) (i + 1)
     else
       arr
-  termination_by insertionSortLoop arr i => arr.size - i
+  termination_by arr.size - i
 stop book declaration
 
 
@@ -713,4 +626,3 @@ expect info {{{ insertionSortStrings }}}
 message
 "#[\"granite\", \"hematite\", \"marble\", \"quartz\"]"
 end expect
-
