examples/Examples/Universes.lean
@@ -139,7 +139,7 @@ message
   α
 at universe level
   2
-it must be smaller than or equal to the inductive datatype universe level
+which is not less than or equal to the inductive type's resulting universe level
   1"
 end expect
 
