examples/first-lake/expected/Greeting.lean
@@ -1,3 +1,3 @@
 -- This module serves as the root of the `Greeting` library.
 -- Import modules here that should be built as part of the library.
-import «Greeting».Basic
+import Greeting.Basic
