functional-programming-lean/src/hello-world/cat.md
@@ -141,9 +141,9 @@ To check whether `feline` works, the first step is to build it with `{{#command 
 First off, when called without arguments, it should emit what it receives from standard input.
 Check that
 ```
-{{#command {feline/2} {feline/2} {echo "It works!" | ./build/bin/feline} }}
+{{#command {feline/2} {feline/2} {echo "It works!" | ./.lake/build/bin/feline} }}
 ```
-emits `{{#command_out {feline/2} {echo "It works!" | ./build/bin/feline} }}`.
+emits `{{#command_out {feline/2} {echo "It works!" | ./.lake/build/bin/feline} }}`.
 
 Secondly, when called with files as arguments, it should print them.
 If the file `test1.txt` contains
@@ -156,20 +156,20 @@ and `test2.txt` contains
 ```
 then the command
 ```
-{{#command {feline/2} {feline/2} {./build/bin/feline test1.txt test2.txt} }}
+{{#command {feline/2} {feline/2} {./.lake/build/bin/feline test1.txt test2.txt} }}
 ```
 should emit
 ```
-{{#command_out {feline/2} {./build/bin/feline test1.txt test2.txt} {feline/2/expected/test12.txt} }}
+{{#command_out {feline/2} {./.lake/build/bin/feline test1.txt test2.txt} {feline/2/expected/test12.txt} }}
 ```
 
 Finally, the `-` argument should be handled appropriately.
 ```
-{{#command {feline/2} {feline/2} {echo "and purr" | ./build/bin/feline test1.txt - test2.txt} }}
+{{#command {feline/2} {feline/2} {echo "and purr" | ./.lake/build/bin/feline test1.txt - test2.txt} }}
 ```
 should yield
 ```
-{{#command_out {feline/2} {echo "and purr" | ./build/bin/feline test1.txt - test2.txt} {feline/2/expected/test1purr2.txt}}}
+{{#command_out {feline/2} {echo "and purr" | ./.lake/build/bin/feline test1.txt - test2.txt} {feline/2/expected/test1purr2.txt}}}
 ```
 
 ## Exercise
